`Transform.runProgram` return an extra `updated` bool result, add analysis cache, and updates to `ProcedureInlining` (#377)
*Description of changes:*

1. The definition of `Transform.runProgram` now returns `(updated, new
program)`, and receives an extra optional arg `allowProcList : Option
(List String)` that makes the transformation only run on specific
procedures.

The goal of this change is to allow the user iteratively apply the
transformation to the specific procedure (e.g., the "main" function)
until there is no change anymore.

2. Add `doInline` fn to Procedure Inlining, let CoreTransformState cache
the result of expensive analysis like CallGraph construction.

In this patch, ProcedureInlining.inlineCallCmd takes a more generic
lambda function `doInline` that receives the calling procedure name as
well as the CallGraph data structure and decide whether to inline or
not.
Since building CallGraph every time is expensive, CallGraph is
incrementally updated after each inlining.
To keep the latest status of CallGraph, we have a new
`CoreTransformState` datatype which tracks analyses cache, and it is the
transformation's responsibility that must invalidate or correctly update
the cache. This mimics what LLVM's passes do.
From the CallGraph, you can check whether e.g., there is only one caller
of some procedure or not.

Also, since we have `CoreTransformState`, more cleaups to the signatures
of transformation functions were possible. The transformation passes
were originally taking an extra source `Program` argument that was being
transformed, but this was awkward because transformations are defined at
the Statement level. This removes the extra argument, and makes
`CoreTransformState` track the currently modifying Program and
Procedure.

3. The `Program.filterProcedures` function is extracted out as a new
transformation called `FilterProcedure`.

The new `Program.filterProcedures` introduced in
https://github.com/strata-org/Strata/pull/375 was extracted out to
`FilterProcedure` because I thought that the correctness of this
`FilterProcedure` can be very nicely described. :) To address the
comment that I left in the pull request, I made `FilterProcedure` a
standalone transform that is not parameteric to other transformations.
Also, there is performance win - combined with the AnalysisCache, now
CallGraph is calculated inside `FilterProcedure` once, reused in
`ProcedureInlining`, then reused in the second `FilterProcedure`!

Also, the proofs in CallElimCorrect is commentized even more.

By submitting this pull request, I confirm that you can use, modify,
copy, and redistribute this contribution, under the terms of your
choice.

@thanhnguyen-aws

Strata/DL/Util/List.lean
@@ -422,4 +422,15 @@ theorem subset_nodup_length {α} {s1 s2: List α} (hn: s1.Nodup) (hsub: s1 ⊆ s
     have hsub1: t ⊆ (l1 ++ l2) := by grind
     grind
 
+
+/-- Deduplicates l and counts the number of occurrences for each element. -/
+def occurrences {α : Type} [DecidableEq α] (l : List α) : List (α × Nat) :=
+  l.dedup.map (λ x => (x, l.count x))
+
+theorem occurrences_len_eq_dedup {α} [DecidableEq α]:
+  ∀ (l : List α), l.dedup.length = l.occurrences.length := by
+  intros l
+  unfold occurrences
+  grind
+
 end List
