Strata/Transform/FilterProcedures.lean
@@ -1,0 +1,53 @@
+/-
+  Copyright Strata Contributors
+
+  SPDX-License-Identifier: Apache-2.0 OR MIT
+-/
+
+import Strata.Transform.CoreTransform
+
+/-! # Erase procedures satisfying specific criteria -/
+
+namespace Core
+namespace FilterProcedures
+
+open Transform
+
+/--
+Filter program to keep only target procedures, applying the specified transform
+to them and pruning away all other procedures.
+Caches the updated CallGraph (which is just dropping unreachable procedure
+entries from the HashMap) to save computation.
+-/
+def run (prog : Program) (targetProcs : List String) :
+    CoreTransformM Program := do
+  let cg := match (← get).cachedAnalyses.callGraph with
+    | .some cg => cg
+    | .none => prog.toProcedureCG
+  let allNeededProcs := (targetProcs ++ cg.getAllCalleesClosure targetProcs).dedup
+  let neededProcsSet := allNeededProcs.toArray.qsort (· < ·)
+  let isNeededProc (procName : String) :=
+    neededProcsSet.binSearch procName (· < ·) |>.isSome
+
+  -- Create a program with target procedures + dependencies.
+  let prunedDecls := prog.decls.filter (fun decl =>
+    match decl with
+    | .proc p _ => isNeededProc (CoreIdent.toPretty p.header.name)
+    | _ => true) -- Keep all non-procedure declarations
+
+  -- Update CallGraph so that filtered out procedures do not appear anymore
+  let filter_cg (m : Std.HashMap String (Std.HashMap String Nat)) :=
+    let m := m.filter (fun k _ => isNeededProc k)
+    m.map (fun _ v => v.filter (fun k _ => isNeededProc k))
+  let cg_new:CallGraph := {
+    callees := filter_cg cg.callees
+    callers := filter_cg cg.callers
+  }
+
+  modify (fun σ => { σ with
+    cachedAnalyses := { σ.cachedAnalyses with callGraph := .some cg_new }})
+
+  return { prog with decls := prunedDecls }
+
+end FilterProcedures
+end Core
